DS: trigger send key event in third protocol step
The sign pred had to be adjusted such that F* can infer that the certify event
was triggered by the server with the actual pub keys of the initiator and responder.
The event pred has been refined for the send key event, such that for all honest
or dishonest principals, the clock count will always be <= second message receive
delay and if the server is honest, a preceeding certify event has been triggered.

denning-sacco/DS.Protocol.fst
@@ -88,7 +88,6 @@ let server_send_msg_2 srv msg1_idx =
       (msg2_idx, new_sess_idx, c_out)
   )
   | _ -> error "[srv_send_m2] wrong message"
-#pop-options
 
 let initiator_send_msg_3 c_in a msg2_idx a_si =
   // get and parse initiator session
@@ -108,22 +107,36 @@ let initiator_send_msg_3 c_in a msg2_idx a_si =
         let verk_srv = get_public_key #ds_preds #now a srv SIG "DS.sig_key" in
 
         // verify initiator and responder certificates
-        if verify #ds_global_usage #now #public #public verk_srv cert_a sig_cert_a then
-          if verify #ds_global_usage #now #public #public verk_srv cert_b sig_cert_b then
+        if verify #ds_global_usage #now #public #public verk_srv cert_a sig_cert_a then (
+          if verify #ds_global_usage #now #public #public verk_srv cert_b sig_cert_b then (
             // parse certificates
             match (parse_sigval cert_a, parse_sigval cert_b) with
             | (Success (CertA a pk_a t), Success (CertB b pk_b t')) -> (
               if t <> t' then error "[i_send_m3] timestamps in initiator and responder certificates do not match"
               else
-                if clock_lte t recv_msg_2_delay c_rm2 then
+                match clock_lte t recv_msg_2_delay c_rm2 with
+                | Success true -> (
                   // validate public key of initiator
                   let pk_a' = get_public_key #ds_preds #now a a PKE "DS.pke_key" in
                   if pk_a <> pk_a' then error "[i_send_m3] wrong initiator public key"
                   else
                     // generate communication key
+                    let prev = now in
                     let (|_,ck|) = rand_gen #ds_preds (readers [P a; P b]) (aead_usage "DS.comm_key") in
 
+                    // trigger event 'send_key'
+                    let event = event_send_key a b srv pk_a pk_b ck t (clock_get c_rm2) in
+                    let now = global_timestamp () in
+                    readers_is_injective srv;
+                    assert(can_flow prev (readers [P srv]) public \/ sign_pred ds_usage_preds prev "DS.sig_key" verk_srv cert_a);
+                    assert(can_flow prev (readers [P srv]) public \/ sign_pred ds_usage_preds prev "DS.sig_key" verk_srv cert_b);
+                    publishable_readers_implies_corruption #prev [P srv];
+                    assert(corrupt_id prev (P srv) \/ sign_pred ds_usage_preds prev "DS.sig_key" verk_srv cert_a);
+                    assert(corrupt_id prev (P srv) \/ sign_pred ds_usage_preds prev "DS.sig_key" verk_srv cert_b);
+                    trigger_event #ds_preds a event;
+
                     // look up sign key of initiator and generate sign nonce
+                    let now = global_timestamp () in
                     let (|_,sigk_a|) = get_private_key #ds_preds #now a SIG "DS.sig_key" in
                     let (|_,n_sig|) = rand_gen #ds_preds (readers [P a]) (nonce_usage "SIG_NONCE") in
 
@@ -141,7 +154,7 @@ let initiator_send_msg_3 c_in a msg2_idx a_si =
                     let c_comm_key = pke_enc #ds_global_usage #now #(readers [P a]) pk_b n_pke ev_comm_key in
 
                     // create and send third message
-                    let msg3 = Msg3 ser_cert_a sig_cert_a ser_cert_b sig_cert_b c_comm_key in
+                    let msg3 = Msg3 cert_a sig_cert_a cert_b sig_cert_b c_comm_key in
                     let ser_msg3 = serialize_msg now msg3 in
 
                     let (|msg3_idx,c_out|) = SR.send #now c_rm2 a b ser_msg3 in
@@ -154,12 +167,15 @@ let initiator_send_msg_3 c_in a msg2_idx a_si =
                     update_session #ds_preds #now a a_si a_vi ser_st;
 
                     (msg3_idx, c_out)
-                else error "[i_send_m3] message has been replayed"
+                )
+                | Success false -> error "[i_send_m3] message has been replayed"
+                | Error e -> error e
             )
             | _ -> error "[i_send_m3] wrong sigvals"
-          else error "[i_send_m3] verification of responder certificate failed"
-        else error "[i_send_m3] verification of initiator certificate failed"
+          ) else error "[i_send_m3] verification of responder certificate failed"
+        ) else error "[i_send_m3] verification of initiator certificate failed"
       )
       | _ -> error "[i_send_m3] wrong message"
   )
   | _ -> error "[i_send_m3] wrong session"
+#pop-options
